language_formal/spark2014_semantics/test.v
@@ -29,8 +29,7 @@ Require Import wellformedness.
  = = = = = = = = = = = = = =*)
 
 Definition f_prime :=
-(* Procedure Body Declaration *)
-      Sproc 3 (
+Procedure 3 (
         mkprocedure_body 4
           (* Procedure Body - Name *)
           (*Test_for_Coq*) 1
@@ -38,32 +37,31 @@ Definition f_prime :=
           (nil)
           (* Procedure Body - Parameters *)
           (nil) 
-          (* Procedure Body - Locally Defined Variables *)
+          (* Procedure Body - Variable Declarations *)
           (
-          mklocal_declaration 5 (*N*) 1 1 (Some (Econst 6 (Ointconst 25))) :: 
-          mklocal_declaration 7 (*Result*) 2 2 None :: 
-          mklocal_declaration 8 (*I*) 3 1 None :: 
-          mklocal_declaration 9 (*X*) 4 1 None :: nil)
-          (* Procedure Body - Body *) (
-            Sseq 10 (
-              Sassign 11 ((*Result*) 2) (Econst 12 (Oboolconst true)) ) ( 
-              Sseq 13 (
-                Sifthen 14 (Ebinop 15 Cle (Evar 16 (*N*) 1) (Econst 17 (Ointconst 1))) (
-                    Sassign 18 ((*Result*) 2) (Econst 19 (Oboolconst false))
+          mkobject_declaration 5 (*N*) 1 1 (Some (E_Literal 6 (Integer_Literal 25))) :: 
+          mkobject_declaration 7 (*Result*) 2 2 None :: 
+          mkobject_declaration 8 (*I*) 3 1 None :: 
+          mkobject_declaration 9 (*X*) 4 1 None :: nil)
+          (* Procedure Body - Statements *) (
+            S_Sequence 10 (
+              S_Assignment 11 ((*Result*) 2) (E_Literal 12 (Boolean_Literal true)) ) ( 
+              S_Sequence 13 (
+                S_If 14 (E_Binary_Operation 15 Less_Than_Or_Equal (E_Identifier 16 (*N*) 1) (E_Literal 17 (Integer_Literal 1))) (
+                    S_Assignment 18 ((*Result*) 2) (E_Literal 19 (Boolean_Literal false))
                   ) ) ( 
-                Sseq 20 (
-                  Sassign 21 ((*I*) 3) (Econst 22 (Ointconst 2)) ) ( 
-                  Swhile 23 (Ebinop 24 Cle (Ebinop 25 Omul (Evar 26 (*I*) 3) (Evar 27 (*I*) 3)) (Evar 28 (*N*) 1)) (
-                      Sseq 29 (
-                        Sassign 30 ((*X*) 4) (Ebinop 31 Odiv (Evar 32 (*N*) 1) (Evar 33 (*I*) 3)) ) ( 
-                        Sseq 34 (
-                          Sifthen 35 (Ebinop 36 Ceq (Evar 37 (*N*) 1) (Ebinop 38 Omul (Evar 39 (*X*) 4) (Evar 40 (*I*) 3))) (
-                              Sassign 41 ((*Result*) 2) (Econst 42 (Oboolconst false))
+                S_Sequence 20 (
+                  S_Assignment 21 ((*I*) 3) (E_Literal 22 (Integer_Literal 2)) ) ( 
+                  S_While_Loop 23 (E_Binary_Operation 24 Less_Than_Or_Equal (E_Binary_Operation 25 Multiply (E_Identifier 26 (*I*) 3) (E_Identifier 27 (*I*) 3)) (E_Identifier 28 (*N*) 1)) (
+                      S_Sequence 29 (
+                        S_Assignment 30 ((*X*) 4) (E_Binary_Operation 31 Divide (E_Identifier 32 (*N*) 1) (E_Identifier 33 (*I*) 3)) ) ( 
+                        S_Sequence 34 (
+                          S_If 35 (E_Binary_Operation 36 Equal (E_Identifier 37 (*N*) 1) (E_Binary_Operation 38 Multiply (E_Identifier 39 (*X*) 4) (E_Identifier 40 (*I*) 3))) (
+                              S_Assignment 41 ((*Result*) 2) (E_Literal 42 (Boolean_Literal false))
                             ) ) ( 
-                          Sassign 43 ((*I*) 3) (Ebinop 44 Oadd (Evar 45 (*I*) 3) (Econst 46 (Ointconst 1))) ) )
+                          S_Assignment 43 ((*I*) 3) (E_Binary_Operation 44 Plus (E_Identifier 45 (*I*) 3) (E_Literal 46 (Integer_Literal 1))) ) )
                     ) ) ) )
-          )
-      ).
+          )).
 
 Check f_prime.
 
@@ -111,7 +109,7 @@ Eval compute in result_with_checks.
      if N <= 1 then
         Result := false;
      end if;
-     I := 0;
+     I := 0; (** coding error ! **)
      while I*I <= N loop
         X := N / I;
         if N = X * I then
@@ -123,8 +121,7 @@ Eval compute in result_with_checks.
  = = = = = = = = = = = = = =*)
 
 Definition f_prime_div_zero :=
-(* Procedure Body Declaration *)
-      Sproc 3 (
+Procedure 3 (
         mkprocedure_body 4
           (* Procedure Body - Name *)
           (*Test_for_Coq1*) 1
@@ -132,29 +129,29 @@ Definition f_prime_div_zero :=
           (nil)
           (* Procedure Body - Parameters *)
           (nil) 
-          (* Procedure Body - Locally Defined Variables *)
+          (* Procedure Body - Variable Declarations *)
           (
-          mklocal_declaration 5 (*N*) 1 2 (Some (Econst 6 (Ointconst 25))) :: 
-          mklocal_declaration 7 (*Result*) 2 3 None :: 
-          mklocal_declaration 8 (*I*) 3 2 None :: 
-          mklocal_declaration 9 (*X*) 4 2 None :: nil)
-          (* Procedure Body - Body *) (
-            Sseq 10 (
-              Sassign 11 ((*Result*) 2) (Econst 12 (Oboolconst true)) ) ( 
-              Sseq 13 (
-                Sifthen 14 (Ebinop 15 Cle (Evar 16 (*N*) 1) (Econst 17 (Ointconst 1))) (
-                    Sassign 18 ((*Result*) 2) (Econst 19 (Oboolconst false))
+          mkobject_declaration 5 (*N*) 1 2 (Some (E_Literal 6 (Integer_Literal 25))) :: 
+          mkobject_declaration 7 (*Result*) 2 3 None :: 
+          mkobject_declaration 8 (*I*) 3 2 None :: 
+          mkobject_declaration 9 (*X*) 4 2 None :: nil)
+          (* Procedure Body - Statements *) (
+            S_Sequence 10 (
+              S_Assignment 11 ((*Result*) 2) (E_Literal 12 (Boolean_Literal true)) ) ( 
+              S_Sequence 13 (
+                S_If 14 (E_Binary_Operation 15 Less_Than_Or_Equal (E_Identifier 16 (*N*) 1) (E_Literal 17 (Integer_Literal 1))) (
+                    S_Assignment 18 ((*Result*) 2) (E_Literal 19 (Boolean_Literal false))
                   ) ) ( 
-                Sseq 20 (
-                  Sassign 21 ((*I*) 3) (Econst 22 (Ointconst 0)) ) ( 
-                  Swhile 23 (Ebinop 24 Cle (Ebinop 25 Omul (Evar 26 (*I*) 3) (Evar 27 (*I*) 3)) (Evar 28 (*N*) 1)) (
-                      Sseq 29 (
-                        Sassign 30 ((*X*) 4) (Ebinop 31 Odiv (Evar 32 (*N*) 1) (Evar 33 (*I*) 3)) ) ( 
-                        Sseq 34 (
-                          Sifthen 35 (Ebinop 36 Ceq (Evar 37 (*N*) 1) (Ebinop 38 Omul (Evar 39 (*X*) 4) (Evar 40 (*I*) 3))) (
-                              Sassign 41 ((*Result*) 2) (Econst 42 (Oboolconst false))
+                S_Sequence 20 (
+                  S_Assignment 21 ((*I*) 3) (E_Literal 22 (Integer_Literal 0)) ) ( 
+                  S_While_Loop 23 (E_Binary_Operation 24 Less_Than_Or_Equal (E_Binary_Operation 25 Multiply (E_Identifier 26 (*I*) 3) (E_Identifier 27 (*I*) 3)) (E_Identifier 28 (*N*) 1)) (
+                      S_Sequence 29 (
+                        S_Assignment 30 ((*X*) 4) (E_Binary_Operation 31 Divide (E_Identifier 32 (*N*) 1) (E_Identifier 33 (*I*) 3)) ) ( 
+                        S_Sequence 34 (
+                          S_If 35 (E_Binary_Operation 36 Equal (E_Identifier 37 (*N*) 1) (E_Binary_Operation 38 Multiply (E_Identifier 39 (*X*) 4) (E_Identifier 40 (*I*) 3))) (
+                              S_Assignment 41 ((*Result*) 2) (E_Literal 42 (Boolean_Literal false))
                             ) ) ( 
-                          Sassign 43 ((*I*) 3) (Ebinop 44 Oadd (Evar 45 (*I*) 3) (Econst 46 (Ointconst 1))) ) )
+                          S_Assignment 43 ((*I*) 3) (E_Binary_Operation 44 Plus (E_Identifier 45 (*I*) 3) (E_Literal 46 (Integer_Literal 1))) ) )
                     ) ) ) )
           )
       ).
@@ -163,7 +160,7 @@ Definition result_1 := f_eval_subprogram 100 nil f_prime_div_zero.
 
 Eval compute in result_1.
 
-Definition run_time_checks_1 := f_check_generator_subprogram nil f_prime.
+Definition run_time_checks_1 := f_check_generator_subprogram nil f_prime_div_zero.
 
 Eval compute in run_time_checks_1.
 
@@ -178,6 +175,86 @@ Eval compute in result_without_checks_1.
 Definition ast_num_inc_1 := f_ast_num_inc_subprogram f_prime_div_zero.
 
 Eval compute in ast_num_inc_1.
+
+(****************
+  - Example 3 -
+ ****************)
+
+(* = = = = = = = = = = = = = =
+  procedure Uninitialized
+  is 
+     N: Integer;  (** N should be initialized before its usage ! **)
+     Result: Boolean;
+     I: Integer;
+     X: Integer;
+  begin
+     Result := true;
+     if N <= 1 then
+        Result := false;
+     end if;
+     I := 0; (** coding error ! **)
+     while I*I <= N loop
+        X := N / I;
+        if N = X * I then
+           Result := false;
+        end if;
+        I := I + 1;
+     end loop;
+  end Test_for_Coq1;
+ = = = = = = = = = = = = = =*)
+
+Definition f_prime_uninitialized :=
+(* Procedure Body Declaration *)
+      Procedure 3 (
+        mkprocedure_body 4
+          (* Procedure Body - Name *)
+          (*Uninitialized*) 1
+          (* Procedure Body - Specification *)
+          (nil)
+          (* Procedure Body - Parameters *)
+          (nil) 
+          (* Procedure Body - Variable Declarations *)
+          (
+          mkobject_declaration 5 (*N*) 1 1 None :: 
+          mkobject_declaration 6 (*Result*) 2 2 None :: 
+          mkobject_declaration 7 (*I*) 3 1 None :: 
+          mkobject_declaration 8 (*X*) 4 1 None :: nil)
+          (* Procedure Body - Statements *) (
+            S_Sequence 9 (
+              S_Assignment 10 ((*Result*) 2) (E_Literal 11 (Boolean_Literal true)) ) ( 
+              S_Sequence 12 (
+                S_If 13 (E_Binary_Operation 14 Less_Than_Or_Equal (E_Identifier 15 (*N*) 1) (E_Literal 16 (Integer_Literal 1))) (
+                    S_Assignment 17 ((*Result*) 2) (E_Literal 18 (Boolean_Literal false))
+                  ) ) ( 
+                S_Sequence 19 (
+                  S_Assignment 20 ((*I*) 3) (E_Literal 21 (Integer_Literal 2)) ) ( 
+                  S_While_Loop 22 (E_Binary_Operation 23 Less_Than_Or_Equal (E_Binary_Operation 24 Multiply (E_Identifier 25 (*I*) 3) (E_Identifier 26 (*I*) 3)) (E_Identifier 27 (*N*) 1)) (
+                      S_Sequence 28 (
+                        S_Assignment 29 ((*X*) 4) (E_Binary_Operation 30 Divide (E_Identifier 31 (*N*) 1) (E_Identifier 32 (*I*) 3)) ) ( 
+                        S_Sequence 33 (
+                          S_If 34 (E_Binary_Operation 35 Equal (E_Identifier 36 (*N*) 1) (E_Binary_Operation 37 Multiply (E_Identifier 38 (*X*) 4) (E_Identifier 39 (*I*) 3))) (
+                              S_Assignment 40 ((*Result*) 2) (E_Literal 41 (Boolean_Literal false))
+                            ) ) ( 
+                          S_Assignment 42 ((*I*) 3) (E_Binary_Operation 43 Plus (E_Identifier 44 (*I*) 3) (E_Literal 45 (Integer_Literal 1))) ) )
+                    ) ) ) )
+          )
+      ).
+
+Definition result_2 := f_eval_subprogram 100 nil f_prime_uninitialized.
+
+Eval compute in result_2.
+
+Definition run_time_checks_2 := f_check_generator_subprogram nil f_prime_uninitialized.
+
+Eval compute in run_time_checks_2.
+
+Definition result_with_checks_2 := f_eval_subprogram_with_checks 100 run_time_checks_2 nil f_prime_uninitialized.
+
+Eval compute in result_with_checks_2.
+
+Definition initialization_result := f_well_defined_subprogram nil f_prime_uninitialized.
+
+Eval compute in initialization_result.
 
 
 (* ======================================================== *)
